Neighborhood/Semantics/Logic/EMKB.lean
@@ -1,0 +1,45 @@
+module
+
+public import Neighborhood.Semantics.Logic.EMB
+public import Neighborhood.Semantics.Logic.EMK
+public import Neighborhood.Semantics.Example.Frame1_3
+public import Neighborhood.Semantics.Example.Frame2_140
+
+@[expose] public section
+
+variable {α : Type u} {A : Formula α}
+
+namespace LogicEMKB
+
+theorem sound {κ} [Nonempty κ] (F : Frame κ) [F.IsMonotonic] [F.HasPropertyK]
+    [F.IsSymmetric] :
+    A ∈ LogicEMKB → F ⊧ A :=
+  Hilbert.sound (by rintro _ ((⟨_, _, rfl⟩ | ⟨_, _, rfl⟩) | ⟨_, rfl⟩) <;> simp)
+
+instance : (@LogicEMKB α).IsConsistent := ⟨by
+  by_contra! hC
+  simpa using LogicEMKB.sound frame_1_2 hC⟩
+
+lemma not_provable_axiomT (a : α) : ∃ A, Axioms.T A ∉ (@LogicEMKB α) := by
+  by_contra! hcon
+  exact frame_1_3.not_valid_axiomT (LogicEMKB.sound frame_1_3 (hcon #a))
+
+lemma not_provable_axiomD (a : α) : ∃ A, Axioms.D A ∉ (@LogicEMKB α) := by
+  by_contra! hcon
+  exact frame_1_3.not_valid_axiomD (LogicEMKB.sound frame_1_3 (hcon #a))
+
+lemma not_provable_axiomP : (Axioms.P : Formula α) ∉ (@LogicEMKB α) := by
+  intro hcon
+  exact frame_1_3.not_valid_axiomP (LogicEMKB.sound frame_1_3 hcon)
+
+lemma not_provable_axiomFour (a : α) : ∃ A, Axioms.Four A ∉ (@LogicEMKB α) := by
+  by_contra! hcon
+  exact frame_2_140.not_valid_axiomFour (LogicEMKB.sound frame_2_140 (hcon #a))
+
+lemma not_provable_axiomFive (a : α) : ∃ A, Axioms.Five A ∉ (@LogicEMKB α) := by
+  by_contra! hcon
+  exact frame_2_140.not_valid_axiomFive (LogicEMKB.sound frame_2_140 (hcon #a))
+
+end LogicEMKB
+
+end
